src/tls/MonotoneMap.fst
@@ -1,3 +1,6 @@
+(*--build-config
+options:--use_hints --fstar_home ../../../FStar --detail_errors --include ../../../FStar/ucontrib/Platform/fst/ --include ../../../FStar/ucontrib/CoreCrypto/fst/ --include ../../../FStar/examples/low-level/crypto/real --include ../../../FStar/examples/low-level/LowCProvider/fst --include ../../../FStar/examples/low-level/crypto --include ../../libs/ffi --include ../../../FStar/ulib/hyperstack --include ideal-flags;
+--*)
 (* A library for monotonic references to partial, dependent maps, with a whole-map invariant *)
 module MonotoneMap
 open FStar.Monotonic.RRef
@@ -17,16 +20,16 @@ type map' (a:Type) (b:a -> Type) =
 type map (a:Type) (b:a -> Type) (inv:map' a b -> Type0) =
   m:map' a b{inv m}
 
-let upd (#a:eqtype) #b (m:map' a b) (x:a) (y:b x) 
-  : Tot (map' a b) 
+let upd (#a:eqtype) #b (m:map' a b) (x:a) (y:b x)
+  : Tot (map' a b)
   = fun z -> if x = z then Some y else m z
 
-let sel #a #b (m:map' a b) (x:a) 
+let sel #a #b (m:map' a b) (x:a)
   : Tot (option (b x))
   = m x
 
-abstract let grows #a #b (m1:map' a b) (m2:map' a b) = 
-  forall x.{:pattern (is_Some (m1 x))}  
+abstract let grows #a #b (m1:map' a b) (m2:map' a b) =
+  forall x.{:pattern (is_Some (m1 x))}
       is_Some (m1 x) ==> is_Some (m2 x) /\ Some.v (m1 x) == Some.v (m2 x)
 
 let grows_reflexive #a #b (m1:map' a b)
@@ -37,37 +40,49 @@ let grows_transitive #a #b (m1:map' a b) (m2:map' a b) (m3:map' a b)
   : Lemma (ensures (grows m1 m2 /\ grows m2 m3 ==> grows m1 m3))
   = ()
 
-let grows_monotone #a #b 
+let grows_monotone #a #b
   : Lemma (monotonic (map' a b) grows)
   = ()
 
 (* Monotone, partial, dependent maps, with a whole-map invariant *)
 type t r a b inv = m_rref r (map a b inv) grows  //maybe grows can include the inv?
 
-let empty_map a b 
-  : Tot (map' a b) 
+let empty_map a b
+  : Tot (map' a b)
   = fun x -> None
 
 type rid = MR.rid
 
-let alloc (#r:rid) #a #b #inv 
+let alloc (#r:rid) #a #b #inv
   : ST (t r a b inv)
        (requires (fun h -> inv (empty_map a b)))
-       (ensures (fun h0 x h1 -> 
-		inv (empty_map a b) /\ 
+       (ensures (fun h0 x h1 ->
+		inv (empty_map a b) /\
 	 	ST.ralloc_post r (empty_map a b) h0 (as_hsref x) h1))
   = grows_monotone #a #b;
     FStar.Monotonic.RRef.m_alloc r (empty_map a b)
 
-let contains #r #a #b #inv (m:t r a b inv) (x:a) (y:b x) (h:HS.mem) 
-  : GTot Type0 
+let defined #r #a #b #inv (m:t r a b inv) (x:a) (h:HS.mem)
+  : GTot Type0
+  = is_Some (sel (m_sel h m) x)
+
+let contains #r #a #b #inv (m:t r a b inv) (x:a) (y:b x) (h:HS.mem)
+  : GTot Type0
   = is_Some (sel (m_sel h m) x) /\ Some.v (sel (m_sel h m) x) == y
+
+let value #r #a #b #inv (m:t r a b inv) (x:a) (h:HS.mem{defined m x h})
+  : GTot (r:b x{contains m x r h})
+  = Some.v (sel (m_sel h m) x)
+
+let fresh #r #a #b #inv (m:t r a b inv) (x:a) (h:HS.mem)
+  : GTot Type0
+  = is_None (sel (m_sel h m) x)
 
 let map_contains #a #b (m1:map' a b) (m2:map' a b) (x:a) (y:b x)
   : Lemma (requires (grows m1 m2))
 	  (ensures (is_Some (m1 x) /\ m1 x == Some y ==> m2 x == Some y))
   = ()
-	  
+
 let contains_stable #r #a #b #inv (m:t r a b inv) (x:a) (y:b x)
   : Lemma (ensures (stable_on_t m (contains m x y)))
   = ()
@@ -75,7 +90,7 @@ let contains_stable #r #a #b #inv (m:t r a b inv) (x:a) (y:b x)
 let extend (#r:rid) (#a:eqtype) (#b:a -> Type) (#inv:(map' a b -> Type0)) (m:t r a b inv) (x:a) (y:b x)
   : ST unit
       (requires (fun h -> let cur = m_sel h m in inv (upd cur x y) /\ sel cur x == None))
-      (ensures (fun h0 u h1 ->		  
+      (ensures (fun h0 u h1 ->
 		  let cur = m_sel h0 m in
 		  let hsref = as_hsref m in
       		  m_contains m h1
@@ -92,16 +107,15 @@ let extend (#r:rid) (#a:eqtype) (#b:a -> Type) (#inv:(map' a b -> Type0)) (m:t r
 let lookup #r #a #b #inv (m:t r a b inv) (x:a)
   : ST (option (b x))
        (requires (fun h -> True))
-       (ensures (fun h0 y h1 -> 
+       (ensures (fun h0 y h1 ->
 		   h0==h1 /\
-		   y == sel (m_sel h1 m) x /\ 
+		   y == sel (m_sel h1 m) x /\
+       (is_None y ==> fresh m x h1) /\
 		   (is_Some y ==> witnessed (contains m x (Some.v y)))))
-  = let y = sel (m_read m) x in 
-    match y with 
+  = let y = sel (m_read m) x in
+    match y with
       | None -> y
-      | Some b -> 
+      | Some b ->
 	contains_stable m x b;
 	witness m (contains m x b);
 	y
-
-
